Simplify src/Nomega.v further

src/HeapState.v
@@ -44,6 +44,42 @@ Definition newHeapState :=
   {| resvs := M.empty _
    ; bytes := M.empty _ |}.
 
+Definition within (addr : N) (len : N) (a : N) : Prop :=
+  addr <= a < addr + len.
+Hint Unfold within.
+
+Definition within_bool (addr : N) (len : N) (a : N) : bool :=
+  ((addr <=? a) && (a <? addr + len))%bool.
+Hint Unfold within_bool.
+
+Definition fits (addr1 len1 addr2 len2 : N) : Prop :=
+  within addr1 len1 addr2 /\ addr2 + len2 <= addr1 + len1.
+Hint Unfold fits.
+
+Definition fits_bool (addr1 len1 addr2 len2 : N) : bool :=
+  (within_bool addr1 len1 addr2 && (addr2 + len2 <=? addr1 + len1))%bool.
+Hint Unfold fits_bool.
+
+Definition overlaps (addr len addr2 len2 : N) : Prop :=
+  addr < addr2 + len2 /\ addr2 < addr + len.
+Hint Unfold overlaps.
+
+Definition overlaps_bool (addr len addr2 len2 : N) : bool :=
+  ((addr <? addr2 + len2) && (addr2 <? addr + len))%bool.
+Hint Unfold overlaps_bool.
+
+Lemma not_overlaps_sym : forall addr1 len1 addr2 len2,
+  ~ overlaps addr1 len1 addr2 len2 <-> ~ overlaps addr2 len2 addr1 len1.
+Proof. autounfold; nomega. Qed.
+
+Corollary not_overlaps_trans : forall a b x y z,
+  z < y -> ~ overlaps a b x y -> ~ overlaps a b x z.
+Proof.
+  unfold not; intros.
+  autounfold in *.
+  apply H0; nomega.
+Qed.
+
 Definition find_free_block (len : Size) (r : M.t Ptr) : Comp Ptr :=
   { addr : N | P.for_all (fun a sz => negb (overlaps_bool a sz addr len)) r }.
 
